\documentclass[12pt]{article}
\usepackage{mlahw}
\begin{document}
\titlehm{3}
\begin{vv286_ms}{1}
\item[(a)]
	\[
	y=\ff{3}{2}-c\ff{1}{x^2},
	\quad
	c\in\R
	\]
\item[(b)]
	\[
	y=\ff{4x+5}{1+8cx+10c}-\ff{3}{2},
	\quad
	c\in\R
	\quad
	\text{or}
	\quad
	y=-\ff{3}{2}
	\]
\item[(c)]
	\[
	y=-\ff{-\cos2x}{2x}e^{-x}+\ff{c}{x}e^{-x},
	\quad
	c\in\R
	\]
\item[(d)]
	\[
	-xy^2+e^y\left( y^2-2y+2 \right)=\rm c
	\quad
	c\in\R
	\]
\item[(e)]
	\[
	y\sin x=\ff{\sin x}{\cos x}+c,
	\quad
	c\in\R
	\]
\item[(f)]
	\[
	y=\ff{x+1}{x-1}(x+c),
	\quad
	c\in\R
	\]
\item[(g)]
	\[
	y+\ff{1}{2}\sin2(x+y)=x+c,
	\quad
	c\in\R
	\]
\item[(h)]
	\[
	\ff{x^2}{2}e^t+xe^{2t}=\rm c
	\quad
	c\in\R
	\]
\item[(i)]
	\[
	x+y=c(x-y)^2
	\quad
	c\in\R
	\quad
	\text{or}
	\quad
	y=x
	\]
\item[(j)]
	\[
	y=-\ln(ce^{-x}-e^{5-x}x),
	\quad
	c\in\R
	\]
\item[(k)]
	\[
	y+\sq{y^2+x^2}=cx^2
	\quad
	c\in\R
	\]	
\item[(l)]
	\[
	(y-1)e^y+e^{-x}+\ff{1}{3}e^{-3}=c,
	\quad
	c\in\R
	\]
\item[(m)]
	\[
	y=\ff{ce^x-x^2}{1+x}-3,
	\quad
	c\in\R
	\]
\item[(n)]
	\[
	\sq{x^2+y^2}e^{\arctan y/x}=c,
	\quad
	c\in\R
	\]
\end{vv286_ms}


\begin{vv286_ms}{2}
\item[(i)]
	Let the incoming light interest the $x$-axis at point
	$D$, the tangent line interest the $x$-axis at point
	$E$, then by geometry we see that $\angle OPD=2\ta$,
	and by parallel line theorem we see that $\phi=\angle
	OPD=2\ta$.\\
	Also, $\tan\ta=\tan\angle OPD={x}/{y}$, and we look
	at the right triangle $\triangle PED$ we see that
	${dy}/{dx}=$\rm the slope of the
	line$=\tan(\pi/2-\ta)$.
\item[(ii)]
	It's just the inverse function theorem:
	\eq{
	\ff{dx}{dy}=\ff{1}{\ff{dy}{dx}}
	=\ff{1}{\tan{\pi/2-\ta}}=\tan\ta
	}
\item[(iii)]
	We use the identity in (i) and (ii):
	\eq
	{
	\ff{x}{y}=\tan2\ta=\ff{2\tan\ta}{1-\tan^2\ta},
	\quad
	\tan\ta=\ff{dx}{dy}
	}
	we rearrange:
	\eq
	{
	xx'^2+2yx'=x
	}
	where the prime is understood as taking derivative
	with respect to $y$, as desired.
\item[(iv)]
	By setting $w=x^2$ we obtain:
	\eq
	{
	\ff{w'^2}{4}+yw'=w
	}
	and set $w'=p$ we solve for:
	\eq
	{
	y=-\ff{p}{2},\quad w=-\ff{p^2}{4}
	}
	which yields no real solution.\\
	Yet the envelope solution gives:
	\eq
	{
	w=cy+\ff{c^2}{4},\quad c\in\R
	}
	substitute $x$ back we obtain:
	\eq
	{
	x^2=cy+\ff{c^2}{4},\quad c\in\R
	}
\item[(v)]
	Indeed, we use {\it paraboloid } mirror and {\it
	parabola} curve to focus the parallel light to a
	single point.
\end{vv286_ms}


\begin{vv286_ms}{3}
\item[(i)]
	\eq
	{
	&y_0=0,\,y_1=\ff{x^3}{3},\quad y_2=\ff{x^3}{3}+\ff{x^7}{63}\\
	&y_3=\ff{x^{15}}{59535}+2\ff{x^{11}}{2079}+\ff{x^7}{67}+\ff{x^3}{3}\\
	&y_4=\ff{x^{31}}{109876902975}+\ff{4x^{27}}{3341878155}+\ff{662x^{23}}{10438212015}
	\\&\quad\quad+\ff{82x^{19}}{37328445}+\ff{13x^{15}}{218295}+\ff{2x^{11}}{2079}+\ff{x^7}{63}+\ff{x^3}{3}
	}
\item[(ii)]
	See attachments.
\end{vv286_ms}


\end{document}


