\input mla
\begin{document}
\titlehm{6}
\begin{vv286_mp}{1}
\item[(i)]
    By Cauchy-Riemann equation:
    \eq
    {
    \pd{u}{x}&=\pd{v}{y}\\
    \pd{u}{y}&=-\pd{v}{x}
    } 
    and this implies:
    \eq
    {
    \dpd{u}{x}&=\spd{v}{x}{y}\\
    \dpd{u}{y}&=-\spd{v}{x}{y}
    }
    thus $u$ is harmonic, a similar procedure shows $v$ is harmonic, 
    this completes the proof.
\item[(ii)]
	One harmonic conjugate:
	\eq
	{
	v=3x^2-3y^2
	}
\end{vv286_mp}

\begin{vv286_ms}{2}
\item[]
	We use the residue to calculate the integral:
	\eq
	{
	\res_{z=a}f(z)=\lim_{z\to a}\ff{1}{z-b}=\ff{1}{a-b}
	}
	Thus by Cauchy Integral formula:
	\eq
	{
	\oint_{\gamma}\ff{1}{(z-a)(z-b)}=2\pi i
	\ff{1}{a-b}
	}
\end{vv286_ms}

\begin{vv286_mp}{3}
\item[]
	We consider the function: $f(z)=e^{iz^2}$, following the
	path given in the question:\\
	$\Gamma_1$: The path on the real line.\\
	$\Gamma_R$: The path rotating the sector.\\
	$\Gamma_2$: The path returning to the origin.\\
	Then on $\Gamma_R$ we have
	\eq
	{
	|e^{iz^2}|=e^{\Re  iz^2}=e^{-\Im  z^2}=e^{-R^2\sin2\ta}	
	}
	where $z=R\cos\ta+iR\sin\ta$. Then using the fact that
	\eq
	{
	\ff{2\ta}{\pi}<\sin\ta
	}
	thus the estimate:
	\eq
	{
	|\int_{\Gamma_R}e^{iz^2}|\leq \ff{\pi}{4}\int_{0}^{\pi/4}e^{-R^2\ta\ff{2}{\pi}}R\,d\ta\le C\ff{1}{R}\to0
	}
	as $R\to\infty$.\\
	On $\Gamma_2$ we use the parametrization:
	$z=(1+i)t$, $t:\ff{\sq{R}}{2}\to 0$, then we have:
	\eq
	{
	\int_{\Gamma_3}f(z)=(1+i)\int_{\ff{\sq2}{2}}^{0}e^{i(2it^2)}\,dt \to-\int_0^{\infty}e^{-2t^2},\,dt=-\ff{\sq{2\pi}}{2}(1+i)
	}
	thus we have:
	\eq
	{
	0=\oint_{\Gamma}f(z)=\int_0^{\infty}e^{ix^2}\,dx+0-\frac{\sq{2\pi}}{2}(1+i)\\
	f(z)=e^{iz^2}=\cos z^2+i\sin z^2
	}
	comparing the real and imaginary part we
	get the desired result.
\end{vv286_mp}

\begin{vv286_ms}{4}
\item[]
	We consider the
	function:$f(z)=e^{iz}-1/(2iz)$
	and the path of integral in the question:\\
	In the inner most semi-circle:
	\eq
	{
	\left|\int_{-C_{\e}}f\right|=\left|\int_{-C_{\e}}\ff{iz+(iz)^2+(iz)^3}{2iz}\,dz\right|=\frac{1}{2}\int_{-C_{\e}}1+|iz|+|o(iz)|
	\le\frac{\pi\e}{2}\to0
	}
	as $\e\to0$.\\
	And the greater semi-circle gives:
	\eq
	{
	\int_{C_{R}}\frac{e^iz-1}{2iz}\,dz=\int\frac{e^{iz}}{2iz}\,dz-
	\int\frac{1}{2iz}\,dz
	=0-\frac{\pi}{2}
	}
	since the first integral vanishes due to Jordan's
	lemma as $R\to\infty$ and the second comes from
	parametrization:$z=e^{i\ta}$.\\
	Finally, the total integral of the closed circle is
	zero, we conclude that:
	\eq
	{
	\oint
	f(z)=\int_{-\infty}^{\infty}\frac{e^{iz}-1}{2iz}\,dz-\frac{\pi}{2}
	=0
	}
	and 
	\begin{align*}
		\frac{e^{ix}-1}{2ix}=\frac{\cos x-1}{x}+\frac{\sin x}{x}
	\end{align*}
	where $x\in\R$ and the first term have no
	contribution to the integration since it's odd.
\end{vv286_ms}
\end{document}
